DenotationalLean/ADeriv.lean
@@ -11,12 +11,9 @@ inductive a_deriv : Aexp -> State -> Nat -> Prop
   | sub {a0 n0 a1 n1 σ} : a_deriv a0 σ n0 -> a_deriv a1 σ n1 -> a_deriv (Aexp.Sub a0 a1) σ (n0-n1)
   | mul {a0 n0 a1 n1 σ} : a_deriv a0 σ n0 -> a_deriv a1 σ n1 -> a_deriv (Aexp.Mul a0 a1) σ (n0*n1)
 
+notation:40 "⟨" a:40 "," σ:40 "⟩" " ~~> " σ':40 => a_deriv a σ σ'
 
-/- example : ⟨(Init + 5) + (7 + 9), σ_0⟩ -> 21 -/
-example : a_deriv
-    ((#"Init" + |5|) + (|7| + |9|))
-    [("Init",0)]
-    21 := by
+example : ⟨(#"Init" + |5|) + (|7| + |9|), [("Init",0)]⟩ ~~> 21 := by
   let σ := [("Init",0)]
   have h0 : State.lookup σ "Init" = 0 := by rfl
   have hi := @a_deriv.loc "Init" σ
@@ -30,12 +27,12 @@ example : a_deriv
   assumption
 
 def a_equiv (a0 a1 : Aexp) : Prop :=
-  ∀ (n : Nat) (σ : State) , (a_deriv a0 σ n) <-> (a_deriv a1 σ n)
+  ∀ (n : Nat) (σ : State) , ⟨a0,σ⟩ ~~> n <-> ⟨a1,σ⟩ ~~> n
 
 /- Proposition 3.3 -/
 
 theorem a_unique (a : Aexp) (σ : State) :
-    ∀ (n0 n1 : Nat) , a_deriv a σ n0 ∧ a_deriv a σ n1 -> n0 = n1 := by
+    ∀ (n0 n1 : Nat) , ⟨a,σ⟩ ~~> n0 ∧ ⟨a,σ⟩ ~~> n1 -> n0 = n1 := by
   induction a <;>
   intro n0 n1 <;> intro ⟨h0,h1⟩ <;>
   cases h0 <;> cases h1 <;> grind
@@ -50,7 +47,7 @@ def a_eval (a : Aexp) (σ : State) : Nat :=
   | .Sub a0 a1 => a_eval a0 σ - a_eval a1 σ
   | .Mul a0 a1 => a_eval a0 σ * a_eval a1 σ
 
-theorem a_eval_deriv (a : Aexp) (σ : State) : a_deriv a σ (a_eval a σ) :=
+theorem a_eval_deriv (a : Aexp) (σ : State) : ⟨a,σ⟩ ~~> a_eval a σ :=
   match a with
   | .Nat _ => a_deriv.num
   | .Loc _ => a_deriv.loc
